Hybrid_Programs/Verification_Examples/Temp_Controller.thy
@@ -4,13 +4,61 @@ theory Temp_Controller
   imports "Hybrid-Verification.Hybrid_Verification"
 begin
 
-lemma fbox_comp_inv_iff: "((I)\<^sub>e \<le> |F] |G] I) \<longleftrightarrow> (((I)\<^sub>e \<le> |F] I) \<and> ((I)\<^sub>e \<le> |G] I))"
-  by (auto simp: fbox_def)
 
-lemma fbox_kcomp_put[wlp]: "fbox (\<langle>\<lambda>s. put\<^bsub>x\<^esub> s v\<rangle> ; F) = fbox (F\<lbrakk>v/x\<rbrakk>)"
-  unfolding fbox_def kcomp_eq
-  by (auto simp: expr_defs assigns_def)
+subsection \<open> Event-triggered thermostat \<close>
 
+dataspace event_triggered_thermostat = 
+  constants 
+    Tmax :: real (* maximum comfortable temp. *)
+    Tmin :: real (* minimum comfortable temp. *)
+    L :: real (* highest temp. when thermostat is on *)
+    K :: real (* freezing factor *)    
+  assumes 
+    Tmin_ge0: "0 < Tmin" 
+    and Tmax_le_Tlim: "Tmax < L"
+    and K_ge0: "K > 0"
+  variables 
+    (* physical *)
+    T :: real      (* temperature *)
+    (* program *)
+    active :: bool (* whether thermostat is on or off *)
+
+context event_triggered_thermostat
+begin 
+
+abbreviation "dyn \<equiv> IF \<not> active 
+  THEN {T` = - K * T | Tmin \<le> T} 
+  ELSE {T` = - K * (T - L) | T \<le> Tmax}"
+
+abbreviation "ctrl \<equiv> 
+  IF \<not> active \<and> T \<le> Tmin THEN active ::= True
+  ELSE IF active \<and> T \<ge> Tmax THEN active ::= False ELSE skip"
+
+lemma event_triggered_therm_flow [local_flow]: "local_flow_on [T \<leadsto> - K * (T - c)] T UNIV UNIV
+  (\<lambda>\<tau>. [T \<leadsto> - exp (-K * \<tau>) * (c - T) + c])"
+  by local_flow_on_auto
+
+lemma thermostat_safe:
+  shows "H{Tmin \<le> T \<and> T \<le> Tmax} 
+    (LOOP (ctrl; dyn) INV (Tmin \<le> T \<and> T \<le> Tmax))
+   {Tmin \<le> T \<and> T \<le> Tmax}"
+  apply intro_loops
+    apply (sequence "Tmin \<le> T \<and> T \<le> Tmax")
+     apply wlp_full
+    apply symbolic_exec
+     apply (wlp_full local_flow: local_flow[where c=0, simplified] simp: field_simps)
+  apply (smt (verit, best) K_ge0 Tmin_ge0 exp_le_one_iff mult_left_le split_mult_pos_le)
+    apply (wlp_full local_flow: local_flow[where c=L, simplified])
+  using K_ge0 Tmin_ge0
+    apply (clarsimp simp: field_simps)
+    apply (smt (verit, best) Tmax_le_Tlim affine_ineq exp_le_one_iff factorL(4) mult_nonneg_nonneg)
+  by expr_auto+
+
+end
+
+
+subsection \<open> Refined thermostat \<close>
+                              
 lemma temp_dyn_down_real_arith:
   assumes "a > 0" and Thyps: "0 < Tmin" "Tmin \<le> T" "T \<le> Tmax"
     and thyps: "0 \<le> (t::real)" "\<forall>\<tau>\<in>{0..t}. \<tau> \<le> - (ln (Tmin / T) / a) "
@@ -58,13 +106,12 @@ proof-
     using Thyps and obs by auto
 qed
 
-
-dataspace original_thermostat = 
+dataspace refined_thermostat = 
   constants 
     Tmax :: real (* maximum comfortable temp. *)
     Tmin :: real (* minimum comfortable temp. *)
     L :: real (* highest temp. when thermostat is on *)
-    K :: real (* freezing rate *)    
+    K :: real (* freezing factor *)    
   assumes 
     Tmin_ge0: "0 < Tmin" 
     and Tmin_le_Tmax: "Tmin + 1 < Tmax" 
@@ -78,118 +125,45 @@ dataspace original_thermostat =
     temp :: real   (* for temperature measurements *)
     active :: bool (* whether thermostat is on or off *)
 
-context original_thermostat
+context refined_thermostat
 begin
 
-(*
-K - heating rate
-
-Inactive
-(1) x(t) = \<theta> * e^{-K*t}
-\<Longrightarrow> x'(t) = -K * \<theta> * e^{-K*t}
-\<Longrightarrow> x'(t) = -K * x(t)
-
-Active
-(2) x(t) = \<theta> * e^{-K*t} + h * (1 - e^{-K*t})
-  = (\<theta> - h) * e^{-K*t} + h
-\<Longrightarrow> x'(t) = -K * \<theta> * e^{-K*t} + K * h *e^{-K*t}
-\<Longrightarrow> x'(t) = - K * (\<theta> - h) * e^{-K*t} 
-   = - K * x(t) - K * h = - K * (x(t) - h)
-
-(1) \<and> (2) \<Longrightarrow> x'(t) = - K * (x(t) - c)
-  where c = if active then h else 0
-*)
-
-subsection \<open> Refined thermostat \<close>
-
-text \<open>
-This thermostat hybrid model refines the literature versions by adding 
-a guard and modifying the control so that it reacts before surpassing the
-comfortable temperatures @{term Tmin} and @{term Tmax}. The consequence
-is that we can prove that the room's temperature @{term T} always remains 
-within the comfortable range @{term "{Tmin--Tmax}"}.
-\<close>
-
-lemma local_flow1: "local_flow_on [T \<leadsto> - K * (T - c), t \<leadsto> 1] (T +\<^sub>L t) UNIV UNIV
-  (\<lambda>\<tau>. [T \<leadsto> - exp (-K * \<tau>) * (c - T) + c, t \<leadsto> \<tau> + t])"
-  by local_flow_on_auto
-
-abbreviation "dyn1 \<equiv> IF \<not> active 
+abbreviation "dyn \<equiv> IF \<not> active 
   THEN {T` = - K * T, t` = 1 | t \<le> - (ln (Tmin/temp))/K} 
   ELSE {T` = - K * (T - L), t` = 1 | t \<le> - (ln ((L - Tmax)/(L - temp)))/K}"
 
-abbreviation "pre_ctrl1 \<equiv> 
+abbreviation "decide \<equiv> 
   IF \<not> active \<and> temp \<le> Tmin + 1 THEN active ::= True
   ELSE IF active \<and> temp \<ge> Tmax - 1 THEN active ::= False ELSE skip"
 
-abbreviation "ctrl1 \<equiv> t ::= 0; temp ::= T; pre_ctrl1"
+abbreviation "ctrl \<equiv> t ::= 0; temp ::= T; decide"
 
-abbreviation "pos_inv \<equiv> (Tmin \<le> $T \<and> $T \<le> Tmax \<and> temp = T \<and> t = 0)\<^sub>e"
-
-lemma thermostat1:
-  "H{Tmin \<le> T \<and> T \<le> Tmax} 
-    (LOOP (ctrl1; dyn1) INV (Tmin \<le> T \<and> T \<le> Tmax))
-   {Tmin \<le> T \<and> T \<le> Tmax}"
-  apply (intro_loops)
-    apply (rule_tac R="pos_inv" in hoare_kcomp)
-     apply (wlp_full)
-    apply (rule hoare_if_then_else)
-     apply (wlp_flow local_flow: local_flow1[where c=0, simplified])
-  apply (clarsimp simp: le_fun_def)
-  using temp_dyn_down_real_arith[OF K_ge0 Tmin_ge0] apply expr_auto
-    apply (wlp_flow local_flow: local_flow1[where c=L, simplified])
-  apply (clarsimp simp: le_fun_def)
-  using temp_dyn_up_real_arith[OF K_ge0 _ _ Tmax_le_Tlim] apply auto[1]
-  using temp_dyn_up_real_arith[OF K_ge0 _ _ Tmax_le_Tlim] 
-  by expr_auto+
-
-
-subsection \<open> Original thermostat \<close>
-
-text \<open>
-This original thermostat model is reactionary. It changes when it detects that
-the temperature of the room is uncomfortable. Thus, the guards directly correspond 
-to the invariant to guarantee the preservation of @{term "Tmin \<le> $T \<and> $T \<le> Tmax"}.
-\<close>
-
-
-abbreviation "dyn2 \<equiv> IF \<not> active 
-  THEN {T` = - K * T | Tmin \<le> T} 
-  ELSE {T` = - K * (T - L) | T \<le> Tmax}"
-
-abbreviation "ctrl2 \<equiv> 
-  IF \<not> active \<and> T \<le> Tmin THEN active ::= True
-  ELSE IF active \<and> T \<ge> Tmax THEN active ::= False ELSE skip"
-
-lemma local_flow2: "local_flow_on [T \<leadsto> - K * (T - c)] T UNIV UNIV
-  (\<lambda>\<tau>. [T \<leadsto> - exp (-K * \<tau>) * (c - T) + c])"
+lemma refined_therm_flow [local_flow]: 
+  "local_flow_on [T \<leadsto> - K * (T - c), t \<leadsto> 1] (T +\<^sub>L t) UNIV UNIV
+  (\<lambda>\<tau>. [T \<leadsto> - exp (-K * \<tau>) * (c - T) + c, t \<leadsto> \<tau> + t])"
   by local_flow_on_auto
 
-lemma thermostat2:
-  assumes le0: "Tmin \<le> Tmax"
-  shows "H{Tmin \<le> T \<and> T \<le> Tmax} 
-    (LOOP (ctrl2; dyn2) INV (Tmin \<le> T \<and> T \<le> Tmax))
+lemma thermostat_safe:
+  "H{Tmin \<le> T \<and> T \<le> Tmax} 
+    (LOOP (ctrl; dyn) INV (Tmin \<le> T \<and> T \<le> Tmax))
    {Tmin \<le> T \<and> T \<le> Tmax}"
   apply (intro_loops)
-    apply (rule_tac R="(Tmin \<le> T \<and> T \<le> Tmax)\<^sup>e" in hoare_kcomp)
+    apply (sequence "Tmin \<le> T \<and> T \<le> Tmax \<and> temp = T \<and> t = 0")
      apply (wlp_full)
-  apply symbolic_exec
-    apply (wlp_full local_flow: local_flow2[where c=0, simplified] simp: field_simps)
-     apply (smt (verit, best) K_ge0 Tmin_ge0 assms div_by_1 exp_ge_zero exp_le_one_iff 
-      max_zero_mult_nonneg_le minus_mult_minus mult.commute mult_eq_0_iff mult_le_0_iff 
-      mult_nonneg_nonneg mult_right_mono_neg nonzero_mult_div_cancel_left one_le_exp_iff 
-      times_divide_eq_left)
-    apply (wlp_full local_flow: local_flow2[where c=L, simplified])
-  using K_ge0 Tmin_ge0 assms
-  apply (clarsimp simp: field_simps)
-  apply (smt (verit, best) Tmax_le_Tlim affine_ineq exp_le_one_iff factorL(4) mult_nonneg_nonneg)
+    apply symbolic_exec
+     apply (wlp_flow local_flow: local_flow[where c=0, simplified])
+     apply (clarsimp simp: le_fun_def)
+  using temp_dyn_down_real_arith[OF K_ge0 Tmin_ge0]
+     apply expr_simp
+    apply (wlp_flow local_flow: local_flow[where c=L, simplified])
+    apply (clarsimp simp: le_fun_def)
+  using temp_dyn_up_real_arith[OF K_ge0 _ _ Tmax_le_Tlim]
   by expr_auto+
 
-lemma "Tmin \<le> Tmax \<Longrightarrow> Tmin \<le> T' \<or> T' \<le> Tmax" for T'::real
-  by linarith
-
-
 end
+
+
+subsection \<open> Time-triggered thermostat \<close>
 
 lemma decr_in_ivl:
   assumes "(K::real) > 0" and "0 < \<epsilon>" and "\<epsilon> < Tmin" and "h > Tmax + \<epsilon>" and "t \<ge> 0"
@@ -200,7 +174,7 @@ proof-
   have "?expr > 0"
     using assms by auto
   hence "exp (- (K * t)) \<ge> 1 - \<epsilon> / T"
-    using key
+    using key  
     by (metis add.inverse_inverse \<open>K > 0\<close> pos_le_minus_divide_eq
         exp_le_cancel_iff exp_ln mult.commute neg_le_iff_le) 
   hence "T - T *  exp (- (K * t)) \<le> \<epsilon>"
@@ -249,14 +223,12 @@ proof-
     by auto
 qed
 
-(* full_exprs *)
-
 dataspace time_triggered_thermostat = 
   constants 
     Tmax :: real (* maximum comfortable temp. *)
     Tmin :: real (* minimum comfortable temp. *)
     L :: real (* highest temp. when thermostat is on *)
-    K :: real (* freezing rate *)    
+    K :: real (* freezing factor *)    
     \<epsilon> :: real (* max increment/decrement of temp per sensing interval *)
   assumes 
     K_ge0: "K > 0"
@@ -291,356 +263,44 @@ abbreviation "dyn \<equiv> IF \<not> active
   THEN {T` = - K * T, t` = 1 | t \<le> - ln (1 - \<epsilon> / temp) / K} 
   ELSE {T` = - K * (T - L), t` = 1 | t \<le> - ln (\<epsilon> / (temp - L) + 1) / K}"
 
-(* Drawing:
-|--------h
-|
-|--------Tmax
-|--------close_to_Tmax
-|
-|
-|--------close_to_Tmin
-|--------Tmin
-*)
 abbreviation "close_to_Tmin \<T> \<equiv> \<T> \<le> Tmin + 1.1 * \<epsilon>"
 abbreviation "close_to_Tmax \<T> \<equiv> \<T> \<ge> Tmax - 1.1 * \<epsilon>"
 
-lemma close_Tmin_not_close_Tmax: "close_to_Tmin \<T> \<Longrightarrow> \<not> close_to_Tmax \<T>"
-proof-
-  assume "close_to_Tmin \<T>"
-  moreover have "1.1 * \<epsilon> < 3 * \<epsilon>"
-    using eps_ge0
-    by auto
-  ultimately show "\<not> close_to_Tmax \<T>"
-    using delta_ge_3eps
-    by linarith
-qed
-
-
-abbreviation "pre_ctrl \<equiv> 
+abbreviation "decide \<equiv> 
   IF \<not> active \<and> close_to_Tmin temp THEN active ::= True
   ELSE IF active \<and> close_to_Tmax temp THEN active ::= False ELSE skip"
 
-abbreviation "ctrl \<equiv> t ::= 0; temp ::= T; pre_ctrl"
+abbreviation "ctrl \<equiv> t ::= 0; temp ::= T; decide"
 
-abbreviation "inv1 \<equiv> (Tmin \<le> $T \<and> $T \<le> Tmax)\<^sub>e"
+expression "pos_inv" is "Tmin \<le> T \<and> T \<le> Tmax \<and> temp = T \<and> t = 0 
+  \<and> (close_to_Tmin temp \<longrightarrow> active) \<and> (close_to_Tmax temp \<longrightarrow> \<not> active)"
 
-abbreviation "pos_inv1 \<equiv> (Tmin \<le> $T \<and> $T \<le> Tmax \<and> temp = T \<and> t = 0 
-  \<and> (close_to_Tmin temp \<longrightarrow> active) \<and> (close_to_Tmax temp \<longrightarrow> \<not> active))\<^sub>e"
-
-(* proof 1 *)
-lemma 
-  "H{Tmin \<le> T \<and> T \<le> Tmax} 
-    (LOOP (ctrl; dyn) INV (Tmin \<le> T \<and> T \<le> Tmax))
-   {Tmin \<le> T \<and> T \<le> Tmax}"
-  apply (rule hoare_loopI)
-    apply (rule_tac R="pos_inv1" in fbox_kcompI)
-  using delta_ge_3eps
-     apply (wlp_full)
-    apply (rule hoare_if_then_else)
-     apply (wlp_full local_flow: local_flow[where c=0, simplified])
-  subgoal 
-    using decr_in_ivl[OF K_ge0 eps_ge0 eps_le_Tmin L_ge_Tmax_eps] 
-    apply clarsimp
-    by (smt (verit) K_ge0 affine_ineq eps_ge0 eps_le_Tmin exp_le_one_iff more_arith_simps(8) zero_le_mult_iff)
-    apply (wlp_full local_flow: local_flow[where c=L, simplified])
-  subgoal
-    using incr_in_ivl[OF K_ge0 eps_ge0 eps_le_Tmin L_ge_Tmax_eps]
-    apply clarsimp
-    by (smt (verit, best) K_ge0 eps_ge0 exp_ge_zero exp_le_one_iff 
-        L_ge_Tmax_eps mult_left_le_one_le mult_sign_intros(1))
-  by expr_auto+
-
-
-(* proof 2 *)
-lemma 
-  "H{Tmin \<le> T \<and> T \<le> Tmax} 
-    (LOOP (ctrl; dyn) INV (Tmin \<le> T \<and> T \<le> Tmax))
-   {Tmin \<le> T \<and> T \<le> Tmax}"
-               apply (intro_loops)
-    apply (subst kcomp_assoc)+
-  apply(subst hoare_kcomp_assign, simp)+
-    apply (subst subst_unrest, simp, expr_simp)+
-    apply (subst subst_id_apply)+
-    apply (subst SEXP_apply)+
-    apply (intro allI)
-  apply (rule_tac R="pos_inv1" in hoare_kcomp)
-  using delta_ge_3eps
-     apply (wlp_full)
-    apply (rule hoare_if_then_else)
-     apply (wlp_full local_flow: local_flow[where c=0, simplified])
-  subgoal 
-    using decr_in_ivl[OF K_ge0 eps_ge0 eps_le_Tmin L_ge_Tmax_eps] 
-    apply clarsimp
-    by (smt (verit) K_ge0 affine_ineq eps_ge0 eps_le_Tmin exp_le_one_iff more_arith_simps(8) zero_le_mult_iff)
-    apply (wlp_full local_flow: local_flow[where c=L, simplified])
-  subgoal
-    using incr_in_ivl[OF K_ge0 eps_ge0 eps_le_Tmin L_ge_Tmax_eps]
-    apply clarsimp
-    by (smt (verit, best) K_ge0 eps_ge0 exp_ge_zero exp_le_one_iff 
-        L_ge_Tmax_eps mult_left_le_one_le mult_sign_intros(1))
-  by expr_auto+
-
-lemma thermostat:
-  "H{Tmin \<le> T \<and> T \<le> Tmax} 
-    (LOOP (ctrl; dyn) INV (Tmin \<le> T \<and> T \<le> Tmax))
-   {Tmin \<le> T \<and> T \<le> Tmax}"
-  apply (wlp_flow local_flow: local_flow[where c=0, simplified])
-  apply (wlp_full local_flow: local_flow[where c=L, simplified])
-  apply (safe; clarsimp?)
-  subgoal
-    by (smt (verit) K_ge0 Tmax_le_L exp_ge_zero exp_le_one_iff mult_left_le_one_le split_mult_pos_le)
-  subgoal for s t
-    using incr_in_ivl[OF K_ge0 eps_ge0 eps_le_Tmin L_ge_Tmax_eps]
-      close_Tmin_not_close_Tmax[of "T<s>"] by auto
-  subgoal for s t
-    by (metis K_ge0 add_mono_thms_linordered_field(5) close_Tmin_not_close_Tmax 
-        decr_in_ivl eps_ge0 eps_le_Tmin less_eq_real_def times_divide_eq_left)
-  subgoal for s t
-    by (smt (verit, ccfv_SIG) K_ge0 eps_le_Tmin exp_ge_zero exp_le_one_iff 
-        mult_left_le_one_le mult_sign_intros(1) zero_le_divide_iff)
-  subgoal for s t
-    by (smt (verit, ccfv_SIG) K_ge0 Tmax_le_L exp_ge_zero exp_le_one_iff 
-        mult_left_le_one_le split_mult_pos_le)
-  subgoal for s t
-    using K_ge0 eps_ge0 eps_le_Tmin L_ge_Tmax_eps incr_in_ivl by blast
-  subgoal for s t
-    using K_ge0 decr_in_ivl eps_ge0 eps_le_Tmin L_ge_Tmax_eps by blast
-  subgoal for s t
-    by (smt (verit, ccfv_SIG) K_ge0 eps_le_Tmin exp_ge_zero exp_le_one_iff 
-        mult_left_le_one_le mult_sign_intros(1) zero_le_divide_iff)
-  subgoal for s t
-    using K_ge0 decr_in_ivl eps_ge0 eps_le_Tmin L_ge_Tmax_eps by blast
-  subgoal for s t
-    by (smt (verit, del_insts) K_ge0 eps_ge0 eps_le_Tmin exp_le_one_iff 
-        mult_left_le_one_le zero_le_mult_iff)
-  subgoal for s t
-    by (meson K_ge0 decr_in_ivl eps_ge0 eps_le_Tmin L_ge_Tmax_eps less_eq_real_def)
-  subgoal for s t
-    by (smt (verit, del_insts) K_ge0 eps_ge0 eps_le_Tmin exp_le_one_iff mult_left_le_one_le zero_le_mult_iff)
-  subgoal for s t
-    by (smt (verit, ccfv_SIG) K_ge0 Tmax_le_L exp_ge_zero exp_le_one_iff 
-        mult_left_le_one_le split_mult_pos_le)
-  subgoal for s t
-    using K_ge0 eps_ge0 eps_le_Tmin L_ge_Tmax_eps incr_in_ivl by blast
-  done
-
-end
-
-thm time_triggered_thermostat_def
- time_triggered_thermostat_def[of 25 20 30 "0.2" "1.6", simplified]
-
-
-(*
-T(\<tau>) = - exp (-K * \<tau>) * (c - T\<^sub>0) + c
-\<and> t(\<tau>) = \<tau> + t\<^sub>0
-\<and> active \<longrightarrow> c = h \<and> \<not> active \<longrightarrow> c = 0
-
-where T\<^sub>0 is the initial value of the temperature that due to our precondition we 
-assume to satisfy Tmin \<le> T\<^sub>0 \<le> Tmax < h.
-Let \<epsilon> > 0 be a temperature increment:
-
-If c=h (i.e. active):
-T\<^sub>0 + \<epsilon> = - exp (-K * \<tau>) * (h - T\<^sub>0) + h
-\<Longrightarrow> \<epsilon> + T\<^sub>0 - h = - exp (-K * \<tau>) * (h - T\<^sub>0)
-\<Longrightarrow> \<epsilon> + T\<^sub>0 - h = exp (-K * \<tau>) * (T\<^sub>0 - h)
-\<Longrightarrow> \<epsilon> / (T\<^sub>0 - h) + 1 = exp (-K * \<tau>)
-\<Longrightarrow> ln (\<epsilon>/(T\<^sub>0 - h) + 1) = -K * \<tau>
-
-We want 1 \<ge> \<epsilon> / (T\<^sub>0 - h) + 1 > 0
-\<Longleftrightarrow> 0 \<ge> \<epsilon> / (T\<^sub>0 - h) > -1
-because in that way, the logarithm exists
-(due to the right inequality) and the 
-magnitudes have physical sense (ln returns a negative due 
-to the left inequality).
-
-Observe that since \<epsilon> > 0 \<and> T\<^sub>0 < h, the lhs
-(0 > \<epsilon> / (T\<^sub>0 - h)) holds. However, we must 
-require \<epsilon> < h - T\<^sub>0 to guarantee the rhs 
-(\<epsilon> / (T\<^sub>0 - h) > -1).
-
-If this holds, then we could define the guard for active as
-\<tau> \<le> -K\<^sup>-\<^sup>1 * ln (\<epsilon>/(T\<^sub>0 - h) + 1) 
-
-Similarly, if c=0 (i.e. if inactive):
-T\<^sub>0 - \<epsilon> = - exp (-K * \<tau>) * (c - T\<^sub>0) + c
-(c = 0) \<Longrightarrow> T\<^sub>0 - \<epsilon> = T\<^sub>0 * exp (-K * \<tau>)
-\<Longrightarrow> 1 - \<epsilon> / T\<^sub>0 = exp (-K * \<tau>)
-\<Longrightarrow> ln (1 - \<epsilon> / T\<^sub>0) = - K * \<tau>
-
-Then we want 1 > 1 - \<epsilon> / T\<^sub>0 > 0
-\<Longleftrightarrow> 0 < \<epsilon> / T\<^sub>0 < 1
-Thus, we need \<epsilon> < T\<^sub>0.
-
-If this holds, then we could define the guard for inactive as
-\<tau> \<le> -K\<^sup>-\<^sup>1 * ln (1 - \<epsilon> / T\<^sub>0)
-
-Now the condition for the control. At most, if the guards 
-are defined as above, the temperature will increase (or 
-decrease) \<epsilon> units. Thus, we can define:
-pre_ctrl \<equiv> 
-  IF \<not> active \<and> temp \<le> Tmin - 1.1 * \<epsilon> THEN active ::= True
-  ELSE IF active \<and> temp \<ge> Tmax - 1.1 * \<epsilon> THEN active ::= False ELSE skip
-
-*)
-
-lemma 
-  assumes "Tmin \<le> (T::real)" and "T \<le> Tmax" and "0 \<le> t"
-    and "\<forall>\<tau>. 0 \<le> \<tau> \<and> \<tau> \<le> t \<longrightarrow> \<tau> \<le> \<epsilon>"
-    and "T \<le> Tmin + exp (- (K * \<epsilon>))"
-    and key: "Tmax - Tmin < L - exp (- (K * \<epsilon>)) * (L - Tmin)"
-    and "exp (-K * \<epsilon>) < (Tmax - Tmin)/Tmax"
-  shows "Tmin \<le> L - exp (- (K * t)) * (L - T)"
-    and "L - exp (- (K * t)) * (L - T) \<le> Tmax"
-proof-
-  have hyps: "Tmin < Tmax" "Tmax < L"
-    sorry
-
-  oops
-
-dataspace thermostat = 
-  constants 
-    Tmax :: real (* maximum comfortable temp. *)
-    Tmin :: real (* minimum comfortable temp. *)
-    L :: real (* highest temp. when thermostat is on *)
-    K :: real (* freezing rate *)    
-    \<epsilon> :: real (* max length of sensing interval *)
-  assumes 
-    K_ge0: "K > 0"
-    and eps_ge0: "\<epsilon> > 0"
-    and Tmax_le_L: "Tmax < L"
-    and Tmin_le: "Tmin < exp (- (K * \<epsilon>)) * Tmax"
-    and Tmax_ge: "Tmax > L - exp (- (K * \<epsilon>)) * (L - Tmin)"
-  variables 
-    (* physical *)
-    T :: real      (* temperature *)
-    t :: real      (* time *)
-    (* program *)
-    temp :: real   (* for temperature measurements *)
-    active :: bool (* whether thermostat is on or off *)
-
-context thermostat
-begin
-
-
-lemma local_flow: "local_flow_on [T \<leadsto> - K * (T - c), t \<leadsto> 1] (T +\<^sub>L t) UNIV UNIV
-  (\<lambda>\<tau>. [T \<leadsto> - exp (-K * \<tau>) * (c - T) + c, t \<leadsto> \<tau> + t])"
-  by local_flow_on_auto
-
-abbreviation "dyn \<equiv> IF \<not> active 
-  THEN {T` = - K * T, t` = 1 | t \<le> \<epsilon>} 
-  ELSE {T` = - K * (T - L), t` = 1 | t \<le> \<epsilon>}"
-
-abbreviation "close_to_Tmin \<T> \<equiv> exp (- (K * \<epsilon>)) * \<T> \<le> Tmin \<and> Tmin \<le> \<T> \<and> L - exp (- (K * \<epsilon>)) * (L - \<T>) < Tmax"
-abbreviation "close_to_Tmax \<T> \<equiv> Tmax < L - exp (- (K * \<epsilon>)) * (L - \<T>) \<and> \<T> \<le> Tmax \<and> Tmin < exp (- (K * \<epsilon>)) * \<T>"
-
-lemma 
-  assumes "close_to_Tmin \<T>"
-    and "close_to_Tmax \<T>"
-    and "Tmin \<le> \<T>" and "\<T> \<le> Tmax"
-  shows "False"
-proof-
-  have "\<And>N. N > 1 \<Longrightarrow> exp (- (N * K * \<epsilon>)) * Tmin \<le> exp (- (N * K * \<epsilon>)) * \<T>"
-    using \<open>Tmin \<le> \<T>\<close> exp_gt_zero mult_le_cancel_left_pos 
-    by blast
-  hence "\<And>N. N > 1 \<Longrightarrow> L + exp (- (N * K * \<epsilon>)) * Tmin - L * exp (- (N * K * \<epsilon>))
-    \<le> L + exp (- (N * K * \<epsilon>)) * \<T> - L * exp (- (N * K * \<epsilon>))"
-    by auto
-  have "False"
-    oops
-
-
-(*
-T\<^sub>1 = c + exp (-K * \<epsilon>) * (T\<^sub>0 - c) 
-   = c + T\<^sub>0 * exp (-K * \<epsilon>) - c * exp (-K * \<epsilon>)
-T\<^sub>2 = c + exp (-K * \<epsilon>) * (c + T\<^sub>0 * exp (-K * \<epsilon>) - c * exp (-K * \<epsilon>) - c)
-   = c + T\<^sub>0 * exp (- 2 * K * \<epsilon>) - c * exp (- 2 * K * \<epsilon>)
-T\<^sub>3 = c + T\<^sub>0 * exp (- 3 * K * \<epsilon>) - c * exp (- 3 * K * \<epsilon>)
-*)
-
-abbreviation "pre_ctrl \<equiv> 
-  IF \<not> active \<and> close_to_Tmin temp THEN active ::= True
-  ELSE IF active \<and> close_to_Tmax temp THEN active ::= False ELSE skip"
-
-abbreviation "ctrl \<equiv> t ::= 0; temp ::= T; pre_ctrl"
-
-abbreviation "pos_inv1 \<equiv> (Tmin \<le> $T \<and> $T \<le> Tmax \<and> temp = T \<and> t = 0
- \<and> (close_to_Tmin temp \<longrightarrow> active) \<and> (close_to_Tmax temp \<longrightarrow> \<not> active))\<^sub>e"
-
-lemma 
+lemma thermostat_safe:
   "H{Tmin \<le> T \<and> T \<le> Tmax} 
     (LOOP (ctrl; dyn) INV (Tmin \<le> T \<and> T \<le> Tmax))
    {Tmin \<le> T \<and> T \<le> Tmax}"
   apply intro_loops
+    apply (sequence pos_inv)
+     apply wlp_full
+  using delta_ge_3eps eps_ge0 apply force
     apply symbolic_exec
-      apply expr_auto[1]
-  subgoal for prev_active
-    apply (wlp_full local_flow: local_flow[where c=L, simplified])
-    apply (hol_intros; clarsimp?)
-    using Tmin_le Tmax_ge
-    apply (smt (verit, del_insts) K_ge0 Tmax_le_L affine_ineq exp_le_one_iff mult_eq_0_iff zero_le_mult_iff)
-    by (smt (verit, del_insts) K_ge0 Tmax_le_L exp_less_cancel_iff mult.commute mult_left_mono)
-    apply symbolic_exec
-  subgoal for prev_active
-    apply (wlp_full local_flow: local_flow[where c=0, simplified])
-    apply (hol_intros; clarsimp?)
-    apply (smt (verit) K_ge0 affine_ineq exp_le_cancel_iff exp_le_one_iff mult.commute mult_eq_0_iff mult_le_cancel_left_pos)
-    using Tmin_le Tmax_ge
-    sorry
-     apply expr_auto[1]
-    apply symbolic_exec
-  subgoal
-    apply (wlp_full local_flow: local_flow[where c=0, simplified])
-    apply (hol_intros; clarsimp?)
-    sorry
-  subgoal
-    sorry
-   apply expr_auto+
-  oops
+     apply (wlp_full local_flow: local_flow[where c=0, simplified])
+     apply (hol_intros)
+    using decr_in_ivl[OF K_ge0 eps_ge0 eps_le_Tmin L_ge_Tmax_eps]
+        apply blast
+       apply (smt (verit) K_ge0 affine_ineq eps_ge0 eps_le_Tmin 
+        exp_le_one_iff more_arith_simps(8) zero_le_mult_iff) 
+      apply (wlp_full local_flow: local_flow[where c=L, simplified])
+      apply (hol_intros)
+       apply (smt (verit, ccfv_SIG) K_ge0 L_ge_Tmax_eps affine_ineq eps_ge0 
+        exp_le_one_iff more_arith_simps(8) zero_le_mult_iff)
+    using incr_in_ivl[OF K_ge0 eps_ge0 eps_le_Tmin L_ge_Tmax_eps]
+    by expr_auto+
 
 end
 
 
 
-(* Other proof attempts
 
-
-  (* apply (subst seq_ifthenelse_distl)+
-    apply (rule hoare_if_then_else)
-     apply(subst forward_assign2, simp, expr_simp)+
-     apply (subst subst_unrest, simp, expr_simp)
-     apply (subst subst_id_apply)+
-  apply (intro allI)
-    apply (rule hoare_if_then_else)
-     apply (wlp_full local_flow: local_flow[where c=0, simplified]) *)
-
-(* apply (subst fbox_kcomp)
-    apply (subst fbox_kcomp)
-    apply (subst fbox_kcomp)
-  thm wlp
-    apply (subst fbox_assign)
-    apply (subst fbox_assign)
-  using subst_comp[of t 0 temp, where Q="fbox dyn inv1"]
-  apply (subst subst_comp) *)
-
-(*
-
-find_theorems "subst_upd" "_ \<dagger> _"
-
-lemma coso: "[x \<leadsto> a] \<dagger> ([y \<leadsto> b] \<dagger> (K x y)) = ([x \<leadsto> a, y \<leadsto> b] \<dagger> (K x y))"
-  unfolding SEXP_def
-  by expr_simp
-
-
-lemma subst_comp[wlp]: "[subst_upd [\<leadsto>] x [\<lambda>\<s>. a]\<^sub>e \<dagger>
-        [[subst_upd [\<leadsto>] y [get\<^bsub>T\<^esub>]\<^sub>e \<dagger>
-          [fbox F
-            [fbox G inv1]\<^sub>e]\<^sub>e]\<^sub>e]\<^sub>e]\<^sub>e = k"
-  using coso
-  unfolding SEXP_def
-  by expr_simp
-
-*)
-
-*)
 
 end
