Hybrid_Programs/Verification_Examples/Bouncing_Ball.thy
@@ -21,10 +21,11 @@ expression safety is "h \<le> H"
 
 expression invariant is "0 \<le> h \<and> v\<^sup>2 \<le> 2*g*(H - h)"
 
-definition "BBall = (h ::= H ; v ::= 0) ; LOOP ((IF h = 0 \<and> v < 0 THEN v ::= -e * v) ; {h` = v, v` = - g | h \<ge> 0}) INV (0 \<le> h \<and> v\<^sup>2 \<le> 2*g*(H - h))"
-
-lemma ball_flow[local_flow]: "local_flow_on [h \<leadsto> v, v \<leadsto> - g] (h +\<^sub>L v) UNIV UNIV (\<lambda>t. [h \<leadsto> - 1 div 2 * g * t ^ 2 + h + t * v, v \<leadsto> - 1 * g * t + v])" 
-  by local_flow_on_auto
+definition "BBall = (h := H ; v := 0); 
+  LOOP (
+    (IF h = 0 \<and> v < 0 THEN v ::= -e * v); 
+    {h` = v, v` = - g | h \<ge> 0}
+  ) INV (0 \<le> h \<and> v\<^sup>2 \<le> 2*g*(H - h))"
 
 text \<open> Proof with differential induction \<close>
 
@@ -48,6 +49,11 @@ lemma bouncing_ball_correct: "H{True} BBall {h \<le> H}"
 
 text \<open> Proof with ODE solution \<close>
 
+lemma ball_flow[local_flow]: 
+  "local_flow_on [h \<leadsto> v, v \<leadsto> - g] (h +\<^sub>L v) UNIV UNIV 
+  (\<lambda>t. [h \<leadsto> - 1 div 2 * g * t ^ 2 + h + t * v, v \<leadsto> - 1 * g * t + v])" 
+  by local_flow_on_auto
+
 lemma bouncing_ball_correct': "H{True} BBall {h \<le> H}"
   unfolding BBall_def 
   apply intro_loops \<comment> \<open> Introduce loop with invariant \<close>
@@ -63,7 +69,7 @@ lemma bouncing_ball_correct': "H{True} BBall {h \<le> H}"
   apply (smt (verit, best) g_pos power2_less_eq_zero_iff zero_compare_simps(4) zero_eq_power2)
   done
 
-text \<open> Alternative proof with ODE solution; could interface with CAS \<close>
+text \<open> Alternative proof supplying the solution; could interface with CAS \<close>
 
 lemma bouncing_ball_correct'': "H{True} BBall {h \<le> H}"
   unfolding BBall_def 
@@ -80,21 +86,15 @@ lemma bouncing_ball_correct'': "H{True} BBall {h \<le> H}"
   apply (smt (verit, best) g_pos power2_less_eq_zero_iff zero_compare_simps(4) zero_eq_power2)
   done
 
-text \<open> Alternative proof with ODE solution; could interface with CAS \<close>
+text \<open> Alternative fully automatic proof \<close>
 
 lemma "H{True} BBall {h \<le> H}"
   unfolding BBall_def 
-  apply intro_loops
-    apply symbolic_exec
-     apply(wlp_full local_flow: ball_flow)
-  apply (clarsimp simp: field_simps)
-  apply (metis bouncing_ball.e_range(2) bouncing_ball_axioms e_range(1) less_eq_real_def linorder_not_less mult.right_neutral mult_le_cancel_left order_trans)
-    apply(wlp_full local_flow: ball_flow)
-  apply (clarsimp simp: field_simps)
-   apply (use H_pos in wlp_simp, expr_auto)
-  by expr_auto
-    (smt (verit, best) g_pos realpow_square_minus_le zero_compare_simps(4))
-
+  apply(wlp_full local_flow: ball_flow)
+    apply (clarsimp simp: field_simps)
+  apply (smt (verit) Groups.mult_ac(2) e_range(1,2) mult_left_le mult_nonneg_nonneg zero_le_square)
+  using H_pos apply linarith
+  by (smt (verit, best) g_pos power2_less_eq_zero_iff zero_compare_simps(4) zero_power2)
 
 end
 
