Hybrid_Programs/Verification_Examples/Pendulum.thy
@@ -1,0 +1,46 @@
+theory Pendulum
+  imports "Hybrid-Verification.Hybrid_Verification"
+
+begin
+
+
+
+dataspace pendulum =
+  constants r :: real
+  variables 
+    x :: real 
+    y :: real
+
+context pendulum
+begin
+
+\<comment> \<open>Verified with annotated dynamics \<close>
+
+abbreviation "pend_flow \<tau> \<equiv> [
+  x \<leadsto> x * cos \<tau> + y * sin \<tau>, 
+  y \<leadsto> - x * sin \<tau> + y * cos \<tau>]"
+
+lemma pendulum_dyn: 
+  "H{\<guillemotleft>r\<guillemotright>\<^sup>2 = ($x)\<^sup>2 + ($y)\<^sup>2} (EVOL pend_flow G U) {\<guillemotleft>r\<guillemotright>\<^sup>2 = ($x)\<^sup>2 + ($y)\<^sup>2}"
+  by (simp add: fbox_g_evol) expr_auto
+
+\<comment> \<open>Verified with Framed derivatives \<close>
+
+lemma pendulum_lie: "H{\<guillemotleft>r\<guillemotright>\<^sup>2 = x\<^sup>2 + y\<^sup>2} {x` = y, y` = - x} {\<guillemotleft>r\<guillemotright>\<^sup>2 = x\<^sup>2 + y\<^sup>2}"
+  by dInduct
+
+\<comment> \<open>Verified with differential invariants as cartesian product \<close>
+
+lemma pendulum_inv: "H{\<guillemotleft>r\<guillemotright>\<^sup>2 = x\<^sup>2 + y\<^sup>2} {(x, y)` = (y, -x)} {\<guillemotleft>r\<guillemotright>\<^sup>2 = x\<^sup>2 + y\<^sup>2}"
+  apply(simp add: hoare_diff_inv_on')
+  apply(rule diff_inv_on_eqI)
+  apply (simp add: var_pair_def)
+  apply clarsimp+
+  apply expr_simp
+  apply (auto intro!: vderiv_intros )
+  done
+
+end
+
+
+end
