Hybrid_Programs/Verification_Examples/Planar_Flight.thy
@@ -1,0 +1,99 @@
+theory Planar_Flight
+  imports "Hybrid-Verification.Hybrid_Verification"
+begin
+
+dataspace planar_flight =
+  constants
+    v\<^sub>o :: real (* own_velocity *)
+    v\<^sub>i :: real (* intruder velocity *)
+  assumes
+    v\<^sub>o_pos: "v\<^sub>o > 0" and
+    v\<^sub>i_pos: "v\<^sub>i > 0"
+  variables (* Coordinates in reference frame of own ship *)
+    x :: real (* Intruder x *)
+    y :: real (* Intruder y *)
+    \<theta> :: real (* Intruder angle *)
+    \<omega> :: real (* Angular velocity *)
+
+context planar_flight
+begin
+
+expression I is "v\<^sub>i * sin \<theta> * x - (v\<^sub>i * cos \<theta> - v\<^sub>o) * y > v\<^sub>o + v\<^sub>i"
+
+expression J is "v\<^sub>i * \<omega> * sin \<theta> * x - v\<^sub>i * \<omega> * cos \<theta> * y 
+                  + v\<^sub>o * v\<^sub>i * cos \<theta> 
+                  > v\<^sub>o * v\<^sub>i + v\<^sub>i * \<omega>"
+
+definition "ctrl = (\<omega> ::= 0; \<questiondown>I?) \<sqinter> (\<omega> ::= 1; \<questiondown>J?)"
+
+definition "plant = {x` = v\<^sub>i * cos \<theta> - v\<^sub>o + \<omega> * y,
+                     y` = v\<^sub>i * sin \<theta> - \<omega> * x,
+                     \<theta>` = -\<omega>}"
+
+definition "flight = (ctrl; plant)\<^sup>*"
+
+lemma flight_safe: "H{x\<^sup>2 + y\<^sup>2 > 0} flight {x\<^sup>2 + y\<^sup>2 > 0}"
+  unfolding flight_def ctrl_def plant_def
+  apply kstar
+  apply (sequence "(\<omega> = 0 \<and> I) \<or> (\<omega> = 1 \<and> J)")
+   apply wlp_full
+  apply split_invariant
+   apply (invariant "\<omega> = 0 \<and> I")
+  apply (dInduct_mega)
+  apply expr_auto
+  apply expr_auto
+  using sum_power2_gt_zero_iff v\<^sub>i_pos v\<^sub>o_pos apply fastforce
+  apply (invariant "\<omega>=1 \<and> J")
+    apply dInduct_mega
+   apply expr_auto
+  apply expr_auto
+  apply (smt (verit) Groups.mult_ac(2) abs_cos_le_one mult_eq_0_iff mult_left_le_one_le v\<^sub>i_pos v\<^sub>o_pos zero_compare_simps(6)
+      zero_le_power2 zero_less_power2)
+  done
+
+end
+
+
+declare [[literal_variables=false]]
+
+lemma diffInvariant:
+  assumes "H{I} g_orbital_on a f (G)\<^sub>e (U)\<^sub>e S t\<^sub>0 {I}" "`P \<longrightarrow> I`"
+          "H{P} g_orbital_on a f (G \<and> I)\<^sub>e (U)\<^sub>e S t\<^sub>0 {Q}"
+  shows "H{P} g_orbital_on a f (G)\<^sub>e (U)\<^sub>e S t\<^sub>0 {Q}"
+  apply (rule diff_cut_on_rule[where C=I])
+  using assms weaken apply fastforce
+  using assms by simp
+
+method dInv for I :: "'st \<Rightarrow> bool" uses facts =
+  (rule diffInvariant[where I="I"],
+   (dInduct_mega facts: facts)[1],
+   (expr_auto)[1])
+
+
+context planar_flight
+begin
+
+lemma flight_safe2: "H{x\<^sup>2 + y\<^sup>2 > 0} flight {x\<^sup>2 + y\<^sup>2 > 0}"
+proof -
+  have ctrl_post: "H{x\<^sup>2 + y\<^sup>2 > 0} ctrl {(\<omega> = 0 \<and> @I) \<or> (\<omega> = 1 \<and> @J)}"
+    unfolding ctrl_def by wlp_full
+
+  have plant_safe_I: "H{\<omega> = 0 \<and> @I} plant {x\<^sup>2 + y\<^sup>2 > 0}"
+    unfolding plant_def apply (dInv "($\<omega> = 0 \<and> @I)\<^sup>e", dWeaken)
+    using v\<^sub>o_pos v\<^sub>i_pos sum_squares_gt_zero_iff by fastforce
+
+  have plant_safe_J: "H{\<omega> = 1 \<and> @J} plant {x\<^sup>2 + y\<^sup>2 > 0}"
+    unfolding plant_def apply (dInv "(\<omega>=1 \<and> @J)\<^sup>e", dWeaken)
+    by (metis add.right_neutral cos_le_one distrib_left less_add_same_cancel2 
+        linorder_not_le linordered_comm_semiring_strict_class.comm_mult_strict_left_mono 
+        mult.right_neutral mult_zero_left not_less_iff_gr_or_eq pos_add_strict 
+        sum_squares_gt_zero_iff v\<^sub>i_pos v\<^sub>o_pos)
+
+    show ?thesis
+    unfolding flight_def apply (intro hoare_kstar_inv hoare_kcomp[OF ctrl_post])
+    by (rule hoare_disj_split[OF plant_safe_I plant_safe_J])
+qed
+
+end
+
+end
