Legacy/Temp_Controller.thy
@@ -1,0 +1,646 @@
+section \<open> Pendulum with force \<close>
+
+theory Temp_Controller
+  imports "Hybrid-Verification.Hybrid_Verification"
+begin
+
+lemma fbox_comp_inv_iff: "((I)\<^sub>e \<le> |F] |G] I) \<longleftrightarrow> (((I)\<^sub>e \<le> |F] I) \<and> ((I)\<^sub>e \<le> |G] I))"
+  by (auto simp: fbox_def)
+
+lemma fbox_kcomp_put[wlp]: "fbox (\<langle>\<lambda>s. put\<^bsub>x\<^esub> s v\<rangle> ; F) = fbox (F\<lbrakk>v/x\<rbrakk>)"
+  unfolding fbox_def kcomp_eq
+  by (auto simp: expr_defs assigns_def)
+
+lemma temp_dyn_down_real_arith:
+  assumes "a > 0" and Thyps: "0 < Tmin" "Tmin \<le> T" "T \<le> Tmax"
+    and thyps: "0 \<le> (t::real)" "\<forall>\<tau>\<in>{0..t}. \<tau> \<le> - (ln (Tmin / T) / a) "
+  shows "Tmin \<le> exp (-a * t) * T" and "exp (-a * t) * T \<le> Tmax"
+proof-
+  have "0 \<le> t \<and> t \<le> - (ln (Tmin / T) / a)"
+    using thyps by auto
+  hence "ln (Tmin / T) \<le> - a * t \<and> - a * t \<le> 0"
+    using assms(1) divide_le_cancel by fastforce
+  also have "Tmin / T > 0"
+    using Thyps by auto
+  ultimately have obs: "Tmin / T \<le> exp (-a * t)" "exp (-a * t) \<le> 1"
+    using exp_ln exp_le_one_iff by (metis exp_less_cancel_iff not_less, simp)
+  thus "Tmin \<le> exp (-a * t) * T"
+    using Thyps by (simp add: pos_divide_le_eq)
+  show "exp (-a * t) * T \<le> Tmax"
+    using Thyps mult_left_le_one_le[OF _ exp_ge_zero obs(2), of T]
+      less_eq_real_def order_trans_rules(23) by blast
+qed
+
+lemma temp_dyn_up_real_arith:
+  assumes "a > 0" and Thyps: "Tmin \<le> T" "T \<le> Tmax" "Tmax < (L::real)"
+    and thyps: "0 \<le> t" "\<forall>\<tau>\<in>{0..t}. \<tau> \<le> - (ln ((L - Tmax) / (L - T)) / a) "
+  shows "L - Tmax \<le> exp (-(a * t)) * (L - T)"
+    and "L - exp (-(a * t)) * (L - T) \<le> Tmax"
+    and "Tmin \<le> L - exp (-(a * t)) * (L - T)"
+proof-
+  have "0 \<le> t \<and> t \<le> - (ln ((L - Tmax) / (L - T)) / a)"
+    using thyps by auto
+  hence "ln ((L - Tmax) / (L - T)) \<le> - a * t \<and> - a * t \<le> 0"
+    using assms(1) divide_le_cancel by fastforce
+  also have "(L - Tmax) / (L - T) > 0"
+    using Thyps by auto
+  ultimately have "(L - Tmax) / (L - T) \<le> exp (-a * t) \<and> exp (-a * t) \<le> 1"
+    using exp_ln exp_le_one_iff by (metis exp_less_cancel_iff not_less)
+  moreover have "L - T > 0"
+    using Thyps by auto
+  ultimately have obs: "(L - Tmax) \<le> exp (-a * t) * (L - T) \<and> exp (-a * t) * (L - T) \<le> (L - T)"
+    by (simp add: pos_divide_le_eq)
+  thus "(L - Tmax) \<le> exp (-(a * t)) * (L - T)"
+    by auto
+  thus "L - exp (-(a * t)) * (L - T) \<le> Tmax"
+    by auto
+  show "Tmin \<le> L - exp (-(a * t)) * (L - T)"
+    using Thyps and obs by auto
+qed
+
+
+dataspace original_thermostat = 
+  constants 
+    Tmax :: real (* maximum comfortable temp. *)
+    Tmin :: real (* minimum comfortable temp. *)
+    L :: real (* highest temp. when thermostat is on *)
+    K :: real (* freezing rate *)    
+  assumes 
+    Tmin_ge0: "0 < Tmin" 
+    and Tmin_le_Tmax: "Tmin + 1 < Tmax" 
+    and Tmax_le_Tlim: "Tmax < L"
+    and K_ge0: "K > 0"
+  variables 
+    (* physical *)
+    T :: real      (* temperature *)
+    t :: real      (* time *)
+    (* program *)
+    temp :: real   (* for temperature measurements *)
+    active :: bool (* whether thermostat is on or off *)
+
+context original_thermostat
+begin
+
+(*
+K - heating rate
+
+Inactive
+(1) x(t) = \<theta> * e^{-K*t}
+\<Longrightarrow> x'(t) = -K * \<theta> * e^{-K*t}
+\<Longrightarrow> x'(t) = -K * x(t)
+
+Active
+(2) x(t) = \<theta> * e^{-K*t} + h * (1 - e^{-K*t})
+  = (\<theta> - h) * e^{-K*t} + h
+\<Longrightarrow> x'(t) = -K * \<theta> * e^{-K*t} + K * h *e^{-K*t}
+\<Longrightarrow> x'(t) = - K * (\<theta> - h) * e^{-K*t} 
+   = - K * x(t) - K * h = - K * (x(t) - h)
+
+(1) \<and> (2) \<Longrightarrow> x'(t) = - K * (x(t) - c)
+  where c = if active then h else 0
+*)
+
+subsection \<open> Refined thermostat \<close>
+
+text \<open>
+This thermostat hybrid model refines the literature versions by adding 
+a guard and modifying the control so that it reacts before surpassing the
+comfortable temperatures @{term Tmin} and @{term Tmax}. The consequence
+is that we can prove that the room's temperature @{term T} always remains 
+within the comfortable range @{term "{Tmin--Tmax}"}.
+\<close>
+
+lemma local_flow1: "local_flow_on [T \<leadsto> - K * (T - c), t \<leadsto> 1] (T +\<^sub>L t) UNIV UNIV
+  (\<lambda>\<tau>. [T \<leadsto> - exp (-K * \<tau>) * (c - T) + c, t \<leadsto> \<tau> + t])"
+  by local_flow_on_auto
+
+abbreviation "dyn1 \<equiv> IF \<not> active 
+  THEN {T` = - K * T, t` = 1 | t \<le> - (ln (Tmin/temp))/K} 
+  ELSE {T` = - K * (T - L), t` = 1 | t \<le> - (ln ((L - Tmax)/(L - temp)))/K}"
+
+abbreviation "pre_ctrl1 \<equiv> 
+  IF \<not> active \<and> temp \<le> Tmin + 1 THEN active ::= True
+  ELSE IF active \<and> temp \<ge> Tmax - 1 THEN active ::= False ELSE skip"
+
+abbreviation "ctrl1 \<equiv> t ::= 0; temp ::= T; pre_ctrl1"
+
+abbreviation "pos_inv \<equiv> (Tmin \<le> $T \<and> $T \<le> Tmax \<and> temp = T \<and> t = 0)\<^sub>e"
+
+lemma thermostat1:
+  "H{Tmin \<le> T \<and> T \<le> Tmax} 
+    (LOOP (ctrl1; dyn1) INV (Tmin \<le> T \<and> T \<le> Tmax))
+   {Tmin \<le> T \<and> T \<le> Tmax}"
+  apply (intro_loops)
+    apply (rule_tac R="pos_inv" in hoare_kcomp)
+     apply (wlp_full)
+    apply (rule hoare_if_then_else)
+     apply (wlp_flow local_flow: local_flow1[where c=0, simplified])
+  apply (clarsimp simp: le_fun_def)
+  using temp_dyn_down_real_arith[OF K_ge0 Tmin_ge0] apply expr_auto
+    apply (wlp_flow local_flow: local_flow1[where c=L, simplified])
+  apply (clarsimp simp: le_fun_def)
+  using temp_dyn_up_real_arith[OF K_ge0 _ _ Tmax_le_Tlim] apply auto[1]
+  using temp_dyn_up_real_arith[OF K_ge0 _ _ Tmax_le_Tlim] 
+  by expr_auto+
+
+
+subsection \<open> Original thermostat \<close>
+
+text \<open>
+This original thermostat model is reactionary. It changes when it detects that
+the temperature of the room is uncomfortable. Thus, the guards directly correspond 
+to the invariant to guarantee the preservation of @{term "Tmin \<le> $T \<and> $T \<le> Tmax"}.
+\<close>
+
+
+abbreviation "dyn2 \<equiv> IF \<not> active 
+  THEN {T` = - K * T | Tmin \<le> T} 
+  ELSE {T` = - K * (T - L) | T \<le> Tmax}"
+
+abbreviation "ctrl2 \<equiv> 
+  IF \<not> active \<and> T \<le> Tmin THEN active ::= True
+  ELSE IF active \<and> T \<ge> Tmax THEN active ::= False ELSE skip"
+
+lemma local_flow2: "local_flow_on [T \<leadsto> - K * (T - c)] T UNIV UNIV
+  (\<lambda>\<tau>. [T \<leadsto> - exp (-K * \<tau>) * (c - T) + c])"
+  by local_flow_on_auto
+
+lemma thermostat2:
+  assumes le0: "Tmin \<le> Tmax"
+  shows "H{Tmin \<le> T \<and> T \<le> Tmax} 
+    (LOOP (ctrl2; dyn2) INV (Tmin \<le> T \<and> T \<le> Tmax))
+   {Tmin \<le> T \<and> T \<le> Tmax}"
+  apply (intro_loops)
+    apply (rule_tac R="(Tmin \<le> T \<and> T \<le> Tmax)\<^sup>e" in hoare_kcomp)
+     apply (wlp_full)
+  apply symbolic_exec
+    apply (wlp_full local_flow: local_flow2[where c=0, simplified] simp: field_simps)
+     apply (smt (verit, best) K_ge0 Tmin_ge0 assms div_by_1 exp_ge_zero exp_le_one_iff 
+      max_zero_mult_nonneg_le minus_mult_minus mult.commute mult_eq_0_iff mult_le_0_iff 
+      mult_nonneg_nonneg mult_right_mono_neg nonzero_mult_div_cancel_left one_le_exp_iff 
+      times_divide_eq_left)
+    apply (wlp_full local_flow: local_flow2[where c=L, simplified])
+  using K_ge0 Tmin_ge0 assms
+  apply (clarsimp simp: field_simps)
+  apply (smt (verit, best) Tmax_le_Tlim affine_ineq exp_le_one_iff factorL(4) mult_nonneg_nonneg)
+  by expr_auto+
+
+lemma "Tmin \<le> Tmax \<Longrightarrow> Tmin \<le> T' \<or> T' \<le> Tmax" for T'::real
+  by linarith
+
+
+end
+
+lemma decr_in_ivl:
+  assumes "(K::real) > 0" and "0 < \<epsilon>" and "\<epsilon> < Tmin" and "h > Tmax + \<epsilon>" and "t \<ge> 0"
+    and T_ivl1: "\<not> T \<le> Tmin + 11 * \<epsilon> / 10"
+    and key: "t \<le> - (ln (1 - \<epsilon> / T) / K)" (is "t \<le> - (ln ?expr / K)")
+  shows "Tmin \<le> exp (- (K * t)) * T"
+proof-
+  have "?expr > 0"
+    using assms by auto
+  hence "exp (- (K * t)) \<ge> 1 - \<epsilon> / T"
+    using key
+    by (metis add.inverse_inverse \<open>K > 0\<close> pos_le_minus_divide_eq
+        exp_le_cancel_iff exp_ln mult.commute neg_le_iff_le) 
+  hence "T - T *  exp (- (K * t)) \<le> \<epsilon>"
+    by (smt (verit, ccfv_SIG) T_ivl1 \<open>0 < \<epsilon>\<close> \<open>\<epsilon> < Tmin\<close> 
+        divide_less_eq_1_pos factor_fracR(2) mult_left_le 
+        mult_pos_pos times_divide_eq_right zero_le_divide_iff)
+  moreover have "T - Tmin \<ge> 1.1 * \<epsilon>"
+    using T_ivl1 
+    by auto
+  ultimately show "Tmin \<le> exp (- (K * t)) * T"
+    using \<open>0 < \<epsilon>\<close> by argo
+qed
+
+lemma incr_in_ivl:
+  assumes "(K::real) > 0" and "0 < \<epsilon>" and "\<epsilon> < Tmin" and "h > Tmax + \<epsilon>" and "t \<ge> 0"
+    and "Tmin \<le> T"
+    and T_ivl2: "\<not> Tmax - 11 * \<epsilon> / 10 \<le> T"
+    and key: "t \<le> - (ln (\<epsilon> / (T - h) + 1) / K)" (is "t \<le> - (ln ?expr / K)")
+  shows "h - exp (- (K * t)) * (h - T) \<le> Tmax"
+proof-
+  have "exp (- (K * t)) * T \<le> T"
+    using assms
+    by force
+  hence "?expr > 0"
+    using \<open>\<epsilon> > 0\<close>
+    by (smt (verit) \<open>h > Tmax + \<epsilon>\<close> T_ivl2 divide_less_eq_1_neg 
+        divide_minus_left divide_nonneg_nonneg) 
+  hence "?expr \<le> exp (- K * t)"
+    using key
+    by (smt (verit, best) \<open>K > 0\<close> divide_minus_left divide_pos_pos exp_ln 
+        factor_fracR(4) ln_ge_iff mult_eq_0_iff mult_minus_left mult_nonneg_nonneg)
+  hence "h - exp (- (K * t)) * (h - T) \<le> h + ?expr * (T - h)"
+    using assms
+    by (smt (verit, ccfv_threshold) divide_pos_pos mult_minus_left 
+        mult_minus_right nonzero_mult_div_cancel_right pos_le_divide_eq)
+  also have "... = h + (\<epsilon> / (T - h) + (T - h)/(T - h)) * (T - h)"
+    by simp
+  also have "... = \<epsilon> + T"
+    by (smt (verit, ccfv_SIG) assms diff_divide_eq_iff divide_cancel_right divide_pos_pos)
+  finally have "h - exp (- (K * t)) * (h - T) \<le> \<epsilon> + T" .
+  moreover have "\<epsilon> + T < 1.1 * \<epsilon> + T"
+    using assms
+    by auto
+  ultimately show ?thesis
+    using T_ivl2
+    by auto
+qed
+
+(* full_exprs *)
+
+dataspace time_triggered_thermostat = 
+  constants 
+    Tmax :: real (* maximum comfortable temp. *)
+    Tmin :: real (* minimum comfortable temp. *)
+    L :: real (* highest temp. when thermostat is on *)
+    K :: real (* freezing rate *)    
+    \<epsilon> :: real (* max increment/decrement of temp per sensing interval *)
+  assumes 
+    K_ge0: "K > 0"
+    and eps_ge0: "\<epsilon> > 0"
+    and eps_le_Tmin: "\<epsilon> < Tmin"
+    and delta_ge_3eps: "Tmax - Tmin > 3 * \<epsilon>" 
+    and L_ge_Tmax_eps: "L > Tmax + \<epsilon>"
+  variables 
+    (* physical *)
+    T :: real      (* temperature *)
+    t :: real      (* time *)
+    (* program *)
+    temp :: real   (* for temperature measurements *)
+    active :: bool (* whether thermostat is on or off *)
+
+context time_triggered_thermostat
+begin
+
+lemma 
+  shows Tmin_le_Tmax: "Tmin < Tmax"
+    and Tmax_le_L: "Tmax < L"
+  using delta_ge_3eps eps_ge0 L_ge_Tmax_eps
+  by linarith+
+
+lemma local_flow: "local_flow_on [T \<leadsto> - K * (T - c), t \<leadsto> 1] (T +\<^sub>L t) UNIV UNIV
+  (\<lambda>\<tau>. [T \<leadsto> - exp (-K * \<tau>) * (c - T) + c, t \<leadsto> \<tau> + t])"
+  by local_flow_on_auto
+
+(* Temperature advances at most \<epsilon> units upwards or downwards 
+before our sensor makes a measurement. *)
+abbreviation "dyn \<equiv> IF \<not> active 
+  THEN {T` = - K * T, t` = 1 | t \<le> - ln (1 - \<epsilon> / temp) / K} 
+  ELSE {T` = - K * (T - L), t` = 1 | t \<le> - ln (\<epsilon> / (temp - L) + 1) / K}"
+
+(* Drawing:
+|--------h
+|
+|--------Tmax
+|--------close_to_Tmax
+|
+|
+|--------close_to_Tmin
+|--------Tmin
+*)
+abbreviation "close_to_Tmin \<T> \<equiv> \<T> \<le> Tmin + 1.1 * \<epsilon>"
+abbreviation "close_to_Tmax \<T> \<equiv> \<T> \<ge> Tmax - 1.1 * \<epsilon>"
+
+lemma close_Tmin_not_close_Tmax: "close_to_Tmin \<T> \<Longrightarrow> \<not> close_to_Tmax \<T>"
+proof-
+  assume "close_to_Tmin \<T>"
+  moreover have "1.1 * \<epsilon> < 3 * \<epsilon>"
+    using eps_ge0
+    by auto
+  ultimately show "\<not> close_to_Tmax \<T>"
+    using delta_ge_3eps
+    by linarith
+qed
+
+
+abbreviation "pre_ctrl \<equiv> 
+  IF \<not> active \<and> close_to_Tmin temp THEN active ::= True
+  ELSE IF active \<and> close_to_Tmax temp THEN active ::= False ELSE skip"
+
+abbreviation "ctrl \<equiv> t ::= 0; temp ::= T; pre_ctrl"
+
+abbreviation "inv1 \<equiv> (Tmin \<le> $T \<and> $T \<le> Tmax)\<^sub>e"
+
+abbreviation "pos_inv1 \<equiv> (Tmin \<le> $T \<and> $T \<le> Tmax \<and> temp = T \<and> t = 0 
+  \<and> (close_to_Tmin temp \<longrightarrow> active) \<and> (close_to_Tmax temp \<longrightarrow> \<not> active))\<^sub>e"
+
+(* proof 1 *)
+lemma 
+  "H{Tmin \<le> T \<and> T \<le> Tmax} 
+    (LOOP (ctrl; dyn) INV (Tmin \<le> T \<and> T \<le> Tmax))
+   {Tmin \<le> T \<and> T \<le> Tmax}"
+  apply (rule hoare_loopI)
+    apply (rule_tac R="pos_inv1" in fbox_kcompI)
+  using delta_ge_3eps
+     apply (wlp_full)
+    apply (rule hoare_if_then_else)
+     apply (wlp_full local_flow: local_flow[where c=0, simplified])
+  subgoal 
+    using decr_in_ivl[OF K_ge0 eps_ge0 eps_le_Tmin L_ge_Tmax_eps] 
+    apply clarsimp
+    by (smt (verit) K_ge0 affine_ineq eps_ge0 eps_le_Tmin exp_le_one_iff more_arith_simps(8) zero_le_mult_iff)
+    apply (wlp_full local_flow: local_flow[where c=L, simplified])
+  subgoal
+    using incr_in_ivl[OF K_ge0 eps_ge0 eps_le_Tmin L_ge_Tmax_eps]
+    apply clarsimp
+    by (smt (verit, best) K_ge0 eps_ge0 exp_ge_zero exp_le_one_iff 
+        L_ge_Tmax_eps mult_left_le_one_le mult_sign_intros(1))
+  by expr_auto+
+
+
+(* proof 2 *)
+lemma 
+  "H{Tmin \<le> T \<and> T \<le> Tmax} 
+    (LOOP (ctrl; dyn) INV (Tmin \<le> T \<and> T \<le> Tmax))
+   {Tmin \<le> T \<and> T \<le> Tmax}"
+               apply (intro_loops)
+    apply (subst kcomp_assoc)+
+  apply(subst hoare_kcomp_assign, simp)+
+    apply (subst subst_unrest, simp, expr_simp)+
+    apply (subst subst_id_apply)+
+    apply (subst SEXP_apply)+
+    apply (intro allI)
+  apply (rule_tac R="pos_inv1" in hoare_kcomp)
+  using delta_ge_3eps
+     apply (wlp_full)
+    apply (rule hoare_if_then_else)
+     apply (wlp_full local_flow: local_flow[where c=0, simplified])
+  subgoal 
+    using decr_in_ivl[OF K_ge0 eps_ge0 eps_le_Tmin L_ge_Tmax_eps] 
+    apply clarsimp
+    by (smt (verit) K_ge0 affine_ineq eps_ge0 eps_le_Tmin exp_le_one_iff more_arith_simps(8) zero_le_mult_iff)
+    apply (wlp_full local_flow: local_flow[where c=L, simplified])
+  subgoal
+    using incr_in_ivl[OF K_ge0 eps_ge0 eps_le_Tmin L_ge_Tmax_eps]
+    apply clarsimp
+    by (smt (verit, best) K_ge0 eps_ge0 exp_ge_zero exp_le_one_iff 
+        L_ge_Tmax_eps mult_left_le_one_le mult_sign_intros(1))
+  by expr_auto+
+
+lemma thermostat:
+  "H{Tmin \<le> T \<and> T \<le> Tmax} 
+    (LOOP (ctrl; dyn) INV (Tmin \<le> T \<and> T \<le> Tmax))
+   {Tmin \<le> T \<and> T \<le> Tmax}"
+  apply (wlp_flow local_flow: local_flow[where c=0, simplified])
+  apply (wlp_full local_flow: local_flow[where c=L, simplified])
+  apply (safe; clarsimp?)
+  subgoal
+    by (smt (verit) K_ge0 Tmax_le_L exp_ge_zero exp_le_one_iff mult_left_le_one_le split_mult_pos_le)
+  subgoal for s t
+    using incr_in_ivl[OF K_ge0 eps_ge0 eps_le_Tmin L_ge_Tmax_eps]
+      close_Tmin_not_close_Tmax[of "T<s>"] by auto
+  subgoal for s t
+    by (metis K_ge0 add_mono_thms_linordered_field(5) close_Tmin_not_close_Tmax 
+        decr_in_ivl eps_ge0 eps_le_Tmin less_eq_real_def times_divide_eq_left)
+  subgoal for s t
+    by (smt (verit, ccfv_SIG) K_ge0 eps_le_Tmin exp_ge_zero exp_le_one_iff 
+        mult_left_le_one_le mult_sign_intros(1) zero_le_divide_iff)
+  subgoal for s t
+    by (smt (verit, ccfv_SIG) K_ge0 Tmax_le_L exp_ge_zero exp_le_one_iff 
+        mult_left_le_one_le split_mult_pos_le)
+  subgoal for s t
+    using K_ge0 eps_ge0 eps_le_Tmin L_ge_Tmax_eps incr_in_ivl by blast
+  subgoal for s t
+    using K_ge0 decr_in_ivl eps_ge0 eps_le_Tmin L_ge_Tmax_eps by blast
+  subgoal for s t
+    by (smt (verit, ccfv_SIG) K_ge0 eps_le_Tmin exp_ge_zero exp_le_one_iff 
+        mult_left_le_one_le mult_sign_intros(1) zero_le_divide_iff)
+  subgoal for s t
+    using K_ge0 decr_in_ivl eps_ge0 eps_le_Tmin L_ge_Tmax_eps by blast
+  subgoal for s t
+    by (smt (verit, del_insts) K_ge0 eps_ge0 eps_le_Tmin exp_le_one_iff 
+        mult_left_le_one_le zero_le_mult_iff)
+  subgoal for s t
+    by (meson K_ge0 decr_in_ivl eps_ge0 eps_le_Tmin L_ge_Tmax_eps less_eq_real_def)
+  subgoal for s t
+    by (smt (verit, del_insts) K_ge0 eps_ge0 eps_le_Tmin exp_le_one_iff mult_left_le_one_le zero_le_mult_iff)
+  subgoal for s t
+    by (smt (verit, ccfv_SIG) K_ge0 Tmax_le_L exp_ge_zero exp_le_one_iff 
+        mult_left_le_one_le split_mult_pos_le)
+  subgoal for s t
+    using K_ge0 eps_ge0 eps_le_Tmin L_ge_Tmax_eps incr_in_ivl by blast
+  done
+
+end
+
+thm time_triggered_thermostat_def
+ time_triggered_thermostat_def[of 25 20 30 "0.2" "1.6", simplified]
+
+
+(*
+T(\<tau>) = - exp (-K * \<tau>) * (c - T\<^sub>0) + c
+\<and> t(\<tau>) = \<tau> + t\<^sub>0
+\<and> active \<longrightarrow> c = h \<and> \<not> active \<longrightarrow> c = 0
+
+where T\<^sub>0 is the initial value of the temperature that due to our precondition we 
+assume to satisfy Tmin \<le> T\<^sub>0 \<le> Tmax < h.
+Let \<epsilon> > 0 be a temperature increment:
+
+If c=h (i.e. active):
+T\<^sub>0 + \<epsilon> = - exp (-K * \<tau>) * (h - T\<^sub>0) + h
+\<Longrightarrow> \<epsilon> + T\<^sub>0 - h = - exp (-K * \<tau>) * (h - T\<^sub>0)
+\<Longrightarrow> \<epsilon> + T\<^sub>0 - h = exp (-K * \<tau>) * (T\<^sub>0 - h)
+\<Longrightarrow> \<epsilon> / (T\<^sub>0 - h) + 1 = exp (-K * \<tau>)
+\<Longrightarrow> ln (\<epsilon>/(T\<^sub>0 - h) + 1) = -K * \<tau>
+
+We want 1 \<ge> \<epsilon> / (T\<^sub>0 - h) + 1 > 0
+\<Longleftrightarrow> 0 \<ge> \<epsilon> / (T\<^sub>0 - h) > -1
+because in that way, the logarithm exists
+(due to the right inequality) and the 
+magnitudes have physical sense (ln returns a negative due 
+to the left inequality).
+
+Observe that since \<epsilon> > 0 \<and> T\<^sub>0 < h, the lhs
+(0 > \<epsilon> / (T\<^sub>0 - h)) holds. However, we must 
+require \<epsilon> < h - T\<^sub>0 to guarantee the rhs 
+(\<epsilon> / (T\<^sub>0 - h) > -1).
+
+If this holds, then we could define the guard for active as
+\<tau> \<le> -K\<^sup>-\<^sup>1 * ln (\<epsilon>/(T\<^sub>0 - h) + 1) 
+
+Similarly, if c=0 (i.e. if inactive):
+T\<^sub>0 - \<epsilon> = - exp (-K * \<tau>) * (c - T\<^sub>0) + c
+(c = 0) \<Longrightarrow> T\<^sub>0 - \<epsilon> = T\<^sub>0 * exp (-K * \<tau>)
+\<Longrightarrow> 1 - \<epsilon> / T\<^sub>0 = exp (-K * \<tau>)
+\<Longrightarrow> ln (1 - \<epsilon> / T\<^sub>0) = - K * \<tau>
+
+Then we want 1 > 1 - \<epsilon> / T\<^sub>0 > 0
+\<Longleftrightarrow> 0 < \<epsilon> / T\<^sub>0 < 1
+Thus, we need \<epsilon> < T\<^sub>0.
+
+If this holds, then we could define the guard for inactive as
+\<tau> \<le> -K\<^sup>-\<^sup>1 * ln (1 - \<epsilon> / T\<^sub>0)
+
+Now the condition for the control. At most, if the guards 
+are defined as above, the temperature will increase (or 
+decrease) \<epsilon> units. Thus, we can define:
+pre_ctrl \<equiv> 
+  IF \<not> active \<and> temp \<le> Tmin - 1.1 * \<epsilon> THEN active ::= True
+  ELSE IF active \<and> temp \<ge> Tmax - 1.1 * \<epsilon> THEN active ::= False ELSE skip
+
+*)
+
+lemma 
+  assumes "Tmin \<le> (T::real)" and "T \<le> Tmax" and "0 \<le> t"
+    and "\<forall>\<tau>. 0 \<le> \<tau> \<and> \<tau> \<le> t \<longrightarrow> \<tau> \<le> \<epsilon>"
+    and "T \<le> Tmin + exp (- (K * \<epsilon>))"
+    and key: "Tmax - Tmin < L - exp (- (K * \<epsilon>)) * (L - Tmin)"
+    and "exp (-K * \<epsilon>) < (Tmax - Tmin)/Tmax"
+  shows "Tmin \<le> L - exp (- (K * t)) * (L - T)"
+    and "L - exp (- (K * t)) * (L - T) \<le> Tmax"
+proof-
+  have hyps: "Tmin < Tmax" "Tmax < L"
+    sorry
+
+  oops
+
+dataspace thermostat = 
+  constants 
+    Tmax :: real (* maximum comfortable temp. *)
+    Tmin :: real (* minimum comfortable temp. *)
+    L :: real (* highest temp. when thermostat is on *)
+    K :: real (* freezing rate *)    
+    \<epsilon> :: real (* max length of sensing interval *)
+  assumes 
+    K_ge0: "K > 0"
+    and eps_ge0: "\<epsilon> > 0"
+    and Tmax_le_L: "Tmax < L"
+    and Tmin_le: "Tmin < exp (- (K * \<epsilon>)) * Tmax"
+    and Tmax_ge: "Tmax > L - exp (- (K * \<epsilon>)) * (L - Tmin)"
+  variables 
+    (* physical *)
+    T :: real      (* temperature *)
+    t :: real      (* time *)
+    (* program *)
+    temp :: real   (* for temperature measurements *)
+    active :: bool (* whether thermostat is on or off *)
+
+context thermostat
+begin
+
+
+lemma local_flow: "local_flow_on [T \<leadsto> - K * (T - c), t \<leadsto> 1] (T +\<^sub>L t) UNIV UNIV
+  (\<lambda>\<tau>. [T \<leadsto> - exp (-K * \<tau>) * (c - T) + c, t \<leadsto> \<tau> + t])"
+  by local_flow_on_auto
+
+abbreviation "dyn \<equiv> IF \<not> active 
+  THEN {T` = - K * T, t` = 1 | t \<le> \<epsilon>} 
+  ELSE {T` = - K * (T - L), t` = 1 | t \<le> \<epsilon>}"
+
+abbreviation "close_to_Tmin \<T> \<equiv> exp (- (K * \<epsilon>)) * \<T> \<le> Tmin \<and> Tmin \<le> \<T> \<and> L - exp (- (K * \<epsilon>)) * (L - \<T>) < Tmax"
+abbreviation "close_to_Tmax \<T> \<equiv> Tmax < L - exp (- (K * \<epsilon>)) * (L - \<T>) \<and> \<T> \<le> Tmax \<and> Tmin < exp (- (K * \<epsilon>)) * \<T>"
+
+lemma 
+  assumes "close_to_Tmin \<T>"
+    and "close_to_Tmax \<T>"
+    and "Tmin \<le> \<T>" and "\<T> \<le> Tmax"
+  shows "False"
+proof-
+  have "\<And>N. N > 1 \<Longrightarrow> exp (- (N * K * \<epsilon>)) * Tmin \<le> exp (- (N * K * \<epsilon>)) * \<T>"
+    using \<open>Tmin \<le> \<T>\<close> exp_gt_zero mult_le_cancel_left_pos 
+    by blast
+  hence "\<And>N. N > 1 \<Longrightarrow> L + exp (- (N * K * \<epsilon>)) * Tmin - L * exp (- (N * K * \<epsilon>))
+    \<le> L + exp (- (N * K * \<epsilon>)) * \<T> - L * exp (- (N * K * \<epsilon>))"
+    by auto
+  have "False"
+    oops
+
+
+(*
+T\<^sub>1 = c + exp (-K * \<epsilon>) * (T\<^sub>0 - c) 
+   = c + T\<^sub>0 * exp (-K * \<epsilon>) - c * exp (-K * \<epsilon>)
+T\<^sub>2 = c + exp (-K * \<epsilon>) * (c + T\<^sub>0 * exp (-K * \<epsilon>) - c * exp (-K * \<epsilon>) - c)
+   = c + T\<^sub>0 * exp (- 2 * K * \<epsilon>) - c * exp (- 2 * K * \<epsilon>)
+T\<^sub>3 = c + T\<^sub>0 * exp (- 3 * K * \<epsilon>) - c * exp (- 3 * K * \<epsilon>)
+*)
+
+abbreviation "pre_ctrl \<equiv> 
+  IF \<not> active \<and> close_to_Tmin temp THEN active ::= True
+  ELSE IF active \<and> close_to_Tmax temp THEN active ::= False ELSE skip"
+
+abbreviation "ctrl \<equiv> t ::= 0; temp ::= T; pre_ctrl"
+
+abbreviation "pos_inv1 \<equiv> (Tmin \<le> $T \<and> $T \<le> Tmax \<and> temp = T \<and> t = 0
+ \<and> (close_to_Tmin temp \<longrightarrow> active) \<and> (close_to_Tmax temp \<longrightarrow> \<not> active))\<^sub>e"
+
+lemma 
+  "H{Tmin \<le> T \<and> T \<le> Tmax} 
+    (LOOP (ctrl; dyn) INV (Tmin \<le> T \<and> T \<le> Tmax))
+   {Tmin \<le> T \<and> T \<le> Tmax}"
+  apply intro_loops
+    apply symbolic_exec
+      apply expr_auto[1]
+  subgoal for prev_active
+    apply (wlp_full local_flow: local_flow[where c=L, simplified])
+    apply (hol_intros; clarsimp?)
+    using Tmin_le Tmax_ge
+    apply (smt (verit, del_insts) K_ge0 Tmax_le_L affine_ineq exp_le_one_iff mult_eq_0_iff zero_le_mult_iff)
+    by (smt (verit, del_insts) K_ge0 Tmax_le_L exp_less_cancel_iff mult.commute mult_left_mono)
+    apply symbolic_exec
+  subgoal for prev_active
+    apply (wlp_full local_flow: local_flow[where c=0, simplified])
+    apply (hol_intros; clarsimp?)
+    apply (smt (verit) K_ge0 affine_ineq exp_le_cancel_iff exp_le_one_iff mult.commute mult_eq_0_iff mult_le_cancel_left_pos)
+    using Tmin_le Tmax_ge
+    sorry
+     apply expr_auto[1]
+    apply symbolic_exec
+  subgoal
+    apply (wlp_full local_flow: local_flow[where c=0, simplified])
+    apply (hol_intros; clarsimp?)
+    sorry
+  subgoal
+    sorry
+   apply expr_auto+
+  oops
+
+end
+
+
+
+(* Other proof attempts
+
+
+  (* apply (subst seq_ifthenelse_distl)+
+    apply (rule hoare_if_then_else)
+     apply(subst forward_assign2, simp, expr_simp)+
+     apply (subst subst_unrest, simp, expr_simp)
+     apply (subst subst_id_apply)+
+  apply (intro allI)
+    apply (rule hoare_if_then_else)
+     apply (wlp_full local_flow: local_flow[where c=0, simplified]) *)
+
+(* apply (subst fbox_kcomp)
+    apply (subst fbox_kcomp)
+    apply (subst fbox_kcomp)
+  thm wlp
+    apply (subst fbox_assign)
+    apply (subst fbox_assign)
+  using subst_comp[of t 0 temp, where Q="fbox dyn inv1"]
+  apply (subst subst_comp) *)
+
+(*
+
+find_theorems "subst_upd" "_ \<dagger> _"
+
+lemma coso: "[x \<leadsto> a] \<dagger> ([y \<leadsto> b] \<dagger> (K x y)) = ([x \<leadsto> a, y \<leadsto> b] \<dagger> (K x y))"
+  unfolding SEXP_def
+  by expr_simp
+
+
+lemma subst_comp[wlp]: "[subst_upd [\<leadsto>] x [\<lambda>\<s>. a]\<^sub>e \<dagger>
+        [[subst_upd [\<leadsto>] y [get\<^bsub>T\<^esub>]\<^sub>e \<dagger>
+          [fbox F
+            [fbox G inv1]\<^sub>e]\<^sub>e]\<^sub>e]\<^sub>e]\<^sub>e = k"
+  using coso
+  unfolding SEXP_def
+  by expr_simp
+
+*)
+
+*)
+
+end
